Proved trav_step_closures_isim for regular read and release rmw cases

src/traversal/SimTravClosure.v
@@ -49,47 +49,45 @@ Module SimTravClosure.
     let (C, I) := tc in
     let C' := I ∩₁ (is_rel lab) ∪₁ codom_rel (⦗C ∪₁ I ∩₁ is_rel lab⦘ ⨾ rmw) in
     let I' := (C ∪₁ I ∩₁ (is_rel lab) ∪₁ codom_rel (⦗C ∪₁ I ∩₁ (is_rel lab)⦘ ⨾ rmw)) ∩₁ W in
-    sim_trav_closure tc = trav_conf_union tc (mkTC C' I'). 
+    sim_trav_closure tc = tc ⊔ (mkTC C' I'). 
   Proof.
     unfold sim_trav_closure. destruct tc as [C I]. simpl.
     apply trav_config_eq_helper; simpl; basic_solver 10.
   Qed.     
 
   Lemma stc_alt (tc: trav_config):
-    sim_trav_closure tc = trav_conf_union tc (mkTC (Cclos tc) (Iclos tc)). 
+    sim_trav_closure tc = tc ⊔ (mkTC (Cclos tc) (Iclos tc)). 
   Proof.
     unfold sim_trav_closure, Iclos, Cclos. destruct tc as [C I]. simpl.
     apply trav_config_eq_helper; simpl; basic_solver 10. 
   Qed.
 
   Lemma stc_tcu_distribute (tc1 tc2: trav_config):
-    sim_trav_closure (trav_conf_union tc1 tc2) =
-    trav_conf_union (sim_trav_closure tc1) (sim_trav_closure tc2).
+    sim_trav_closure (tc1 ⊔ tc2) =
+    (sim_trav_closure tc1) ⊔ (sim_trav_closure tc2).
   Proof. 
-    unfold sim_trav_closure, trav_conf_union.
+    unfold sim_trav_closure, trav_config_union.
     destruct tc1 as [C1 I1], tc2 as [C2 I2]. simpl.
     apply trav_config_eq_helper; simpl; basic_solver 10. 
   Qed.
 
   Lemma tcu_assoc (tc1 tc2 tc3: trav_config):
-    trav_conf_union (trav_conf_union tc1 tc2) tc3 =
-    trav_conf_union tc1 (trav_conf_union tc2 tc3).
+     (tc1 ⊔ tc2) ⊔ tc3 = tc1 ⊔ (tc2 ⊔ tc3).
   Proof.
-    destruct tc1, tc2, tc3. unfold trav_conf_union.
+    destruct tc1, tc2, tc3. unfold trav_config_union.
     apply trav_config_eq_helper; simpl; basic_solver.
   Qed.
 
   Lemma tcu_symm (tc1 tc2: trav_config):
-    trav_conf_union tc1 tc2 = 
-    trav_conf_union tc2 tc1. 
+    tc1 ⊔ tc2 = tc2 ⊔ tc1. 
   Proof.
-    destruct tc1, tc2. unfold trav_conf_union.
+    destruct tc1, tc2. unfold trav_config_union.
     apply trav_config_eq_helper; simpl; basic_solver.
   Qed.
 
   (* Lemma sim_trav_step_closure (tc tc': trav_config) *)
-  (*       (SIM_TRAV_STEP: (sim_trav_step G sc)^? tc (trav_conf_union tc tc')): *)
-  (*   (sim_trav_step G sc)^? (sim_trav_closure tc) (trav_conf_union (sim_trav_closure tc) (sim_trav_closure tc')). *)
+  (*       (SIM_TRAV_STEP: (sim_trav_step G sc)^? tc (trav_config_union tc tc')): *)
+  (*   (sim_trav_step G sc)^? (sim_trav_closure tc) (trav_config_union (sim_trav_closure tc) (sim_trav_closure tc')). *)
   (* Proof.  *)
   (*   destruct SIM_TRAV_STEP. *)
   (*   2: { red in H. desc. right. exists thread. inversion H; subst. *)
@@ -128,25 +126,14 @@ Module SimTravClosure.
     all: (rewrite COVEQ || rewrite ISSEQ); basic_solver.
   Qed.
 
-  Lemma itrav_step_eq (tc1 tc2 tc1' tc2': trav_config) (e: actid)
+  Lemma isim_trav_step_more (tc1 tc2 tc1' tc2': trav_config) (thread: thread_id)
         (EQUIV1: same_trav_config tc1 tc1') (EQUIV2: same_trav_config tc2 tc2')
-        (STEP: (itrav_step G sc) e tc1 tc2):
-    (itrav_step G sc) e tc1' tc2'.
+        (STEP: isim_trav_step G sc thread tc1 tc2):
+    isim_trav_step G sc thread tc1' tc2'.
   Proof.
-    red in EQUIV1, EQUIV2. desc.
-    red in STEP. desf.
-    { left. splits.
-      { intros ?. destruct NEXT. by apply EQUIV1. }
-      { eapply coverable_more; eauto. by apply same_tc_Symmetric. }
-      { rewrite <- EQUIV2, <- EQUIV1. auto. }
-      { rewrite <- EQUIV0, <- EQUIV3. auto. }
-    }
-    right. splits.
-    { intros ?. destruct NISS. by apply EQUIV3. }
-    { eapply issuable_more; eauto. by apply same_tc_Symmetric. }
-    { rewrite <- EQUIV2, <- EQUIV1. auto. }
-    { rewrite <- EQUIV0, <- EQUIV3. auto. }
-  Qed.     
+    replace tc1' with tc1; [replace tc2' with tc2| ]; auto.
+    all: destruct EQUIV1, EQUIV2; apply trav_config_eq_helper; auto.
+  Qed. 
 
   Lemma itrav_step_mon_ext' e
         (C1 I1 C2 I2 C' I': actid -> Prop)
@@ -208,17 +195,183 @@ Module SimTravClosure.
       erewrite trav_config_eq_helper'; [| simpl; by rewrite <- C_ALT | reflexivity].
       simpl.
       eapply itrav_step_mon_ext with (C' := C') (I' := I') in TS as [? | ?].
-      2: { eapply itrav_step_eq; [| | by apply H0]; basic_solver. }
+      2: { eapply itrav_step_more; [reflexivity| .. | apply H0].
+           all: by apply same_tc_Symmetric. }
       inversion H0. destruct H. rewrite H2. basic_solver. }
   Admitted.
 
   Lemma isim_trav_step_mon_tcu thread
         (tc1 tc2 tc': trav_config)
         (STEP: isim_trav_step G sc thread tc1 tc2):
-    (isim_trav_step G sc thread)^? (trav_conf_union tc1 tc') (trav_conf_union tc2 tc').
+    (isim_trav_step G sc thread)^? (tc1 ⊔ tc') (tc2 ⊔ tc').
   Proof. 
     destruct tc1, tc2, tc'. apply isim_trav_step_mon; auto. 
   Qed.
+
+  Lemma tcu_same_equiv (tc1 tc2 tc1' tc2': trav_config)
+        (SAME1: same_trav_config tc1 tc1') (SAME2: same_trav_config tc2 tc2'):
+    tc1 ⊔ tc2 = tc1' ⊔ tc2'.
+  Proof.
+    red in SAME1, SAME2. destruct tc1, tc2, tc1', tc2'. desc. simpl in *.
+    apply trav_config_eq_helper; simpl; apply set_equiv_union; auto.
+  Qed.
+
+  Definition empty_tc := mkTC ∅ ∅.
+
+  Lemma tcu_empty_l (tc: trav_config):
+    tc ⊔ empty_tc = tc.
+  Proof.
+    unfold trav_config_union. apply trav_config_eq_helper; simpl; basic_solver.
+  Qed.
+
+  Lemma functional_codom {A: Type} (r: relation A) (a: A)
+        (FUN: functional r)
+        (DOMa: dom_rel r a):
+    exists a', codom_rel (⦗eq a⦘ ⨾ r) ≡₁ eq a'.
+  Proof.
+    destruct DOMa as [a' Raa']. exists a'. split; [| basic_solver].  
+    intros x [a_ Ra_x%seq_eqv_l]. desc. subst.
+    eapply FUN; eauto.
+  Qed.
+
+  Lemma trav_step_closures_isim WF CONS
+        (tc tc': trav_config)
+        (COH: tc_coherent G sc tc)
+        (COH': tc_coherent G sc tc')
+        (TRAV_STEP: trav_step G sc tc tc'):
+    (sim_trav_step G sc)^? (sim_trav_closure tc) (sim_trav_closure tc').
+  Proof.
+    assert (forall tc C1 I1 C2 I2
+              (COV: covered tc ≡₁ C1 ∪₁ C2)
+              (ISS: issued tc ≡₁ I1 ∪₁ I2),
+               tc = (mkTC C1 I1) ⊔ (mkTC C2 I2)) as TCU_HELPER.
+    { ins. unfold trav_config_union. apply trav_config_eq_helper; simpl; auto. }
+    (* cdes TRAV_STEP. *)
+    
+    red in TRAV_STEP. desc. 
+    enough ((isim_trav_step G sc (tid e))^? (sim_trav_closure tc) (sim_trav_closure tc')) as ISIM.
+    { destruct ISIM; [basic_solver| ]. right. by exists (tid e). }
+    cdes TRAV_STEP. desf. 
+    
+    desf.
+    { pose proof (lab_rwf lab e) as LABe. des.
+      { remember (mkTC (eq e) ∅) as tc''. 
+
+        assert (tc' = tc ⊔ tc'') as TC'_UNION.
+        { subst tc''. apply trav_config_eq_helper; simpl; auto.
+          generalize ISSEQ. basic_solver. }
+        
+        assert (sim_trav_closure tc'' =
+                mkTC (eq e ∪₁ codom_rel (⦗eq e⦘ ⨾ rmw))
+                     (codom_rel (⦗eq e⦘ ⨾ rmw))) as TC''.
+        { apply trav_config_eq_helper; subst tc''; simpl.
+          { by rewrite !set_inter_empty_l, !set_union_empty_r. }
+          rewrite !set_inter_empty_l, !set_union_empty_r, !set_union_empty_l.
+          rewrite set_inter_union_l. erewrite set_equiv_union.
+          3: { apply set_inter_absorb_r.
+               rewrite wf_rmwD; auto; basic_solver. }
+          2: { apply set_subset_empty_r. type_solver. }
+          basic_solver. }
+
+        forward eapply eq_trans as TC''_UNION; [apply TC''| | ]. 
+        { eapply TCU_HELPER; simpl; [reflexivity| ]. 
+          symmetry. apply set_union_empty_l. }
+
+        rewrite TC'_UNION, stc_tcu_distribute.
+        rewrite TC''_UNION.
+        
+        destruct (classic (dom_rel rmw e)) as [RMWr | NRMWr].
+        2: { assert (codom_rel (⦗eq e⦘ ⨾ rmw) ≡₁ ∅) as NOADD.
+             { generalize NRMWr. basic_solver. } 
+             
+             (* TODO: declare instances for same_trav_config *)
+             rewrite <- tcu_assoc. erewrite tcu_same_equiv with (tc2' := empty_tc).
+             2: { by apply same_tc_Symmetric. }
+             2: { split; auto. }   
+             rewrite tcu_empty_l. rewrite <- Heqtc''. 
+             rewrite !stc_alt.
+             rewrite tcu_assoc, tcu_symm with (tc2 := tc''), <- tcu_assoc.
+             apply isim_trav_step_mon_tcu.
+             subst tc''. destruct tc as [C I], tc' as [C' I']. simpl in *.
+             unfold trav_config_union. simpl.
+             erewrite trav_config_eq_helper'; cycle 1. 
+             { simpl. reflexivity. }
+             { simpl. apply set_union_empty_r. }
+             eapply read_trav_step; auto. simpl.
+             eapply itrav_step_more; eauto; [done| ].
+             red. split; simpl; symmetry; auto. }
+
+        rename e into r.
+        forward eapply (functional_codom rmw r) as [w RMWD]; auto using wf_rmwf.
+        pose proof (proj2 RMWD) as RMW. red in RMW. specialize (RMW w eq_refl).
+        red in RMW. desc. apply seq_eqv_l in RMW as [<- RMW].          
+
+        assert (E w /\ W w) as [Ew Ww].
+        { eapply same_relation_exp in RMW.
+          2: { rewrite wf_rmwD, wf_rmwE; auto. }
+          unfolder in RMW. desc. subst. auto. } 
+        (* TODO: get rid of previous excessive split of tc'' *)
+        erewrite <- TCU_HELPER with (tc := sim_trav_closure tc''); cycle 1.
+        1,2: rewrite TC''; simpl; basic_solver.
+        rewrite TC''.
+        rewrite !stc_alt.
+
+        destruct (classic (is_rel lab w)) as [RELw | NRELw].
+        { rewrite <- TC''. 
+          rewrite tcu_assoc, tcu_symm with (tc2 := sim_trav_closure tc''), <- tcu_assoc.
+          apply isim_trav_step_mon_tcu.
+          rewrite TC''. 
+          destruct tc as [C I] eqn:TC, tc' as [C' I'] eqn:TC'. simpl in *.
+          unfold trav_config_union. simpl. 
+          eapply isim_trav_step_more; [apply same_tc_Reflexive| ..]. 
+          { erewrite trav_config_eq_helper'; [apply same_tc_Reflexive| ..]; simpl.
+            { rewrite RMWD, <- set_unionA. reflexivity. }
+            rewrite RMWD. reflexivity. }
+          assert (~ I w) as NIw. 
+          { intros ISSw. cdes COH. apply II in ISSw.
+            red in ISSw. apply proj1, proj2 in ISSw.
+            red in ISSw. specialize (ISSw r). specialize_full ISSw; [| done]. 
+            apply dom_rel_fun_alt. red. repeat left.
+            apply seq_eqv_r. unfolder; splits; auto.
+            by apply rmw_in_sb. }
+          assert (~ C w) as NCw.
+          { intros Cw. destruct NIw.
+            forward eapply (w_covered_issued COH (conj Ww Cw)). auto. }
+
+          assert (dom_cond sb (C ∪₁ eq r) w) as DC_SBw. 
+          { unfolder. ins. desc. subst z y.
+            destruct (classic (x = r)) as [-> | ]; [tauto| ]. left.
+            apply wf_rmwi in RMW as [SBrw IMMrw]; auto.
+            assert ((sb ⨾ ⦗covered tc'⦘) x r) as SBxr.
+            { apply seq_eqv_r. split.
+              2: { subst. simpl. apply COVEQ. basic_solver. } 
+              eapply sb_semi_total_r in SBrw; eauto.
+              2: { eapply read_or_fence_is_not_init; eauto. }
+              des; auto. edestruct IMMrw; eauto. }
+            forward eapply (@dom_sb_covered G) with (T := tc') as SB_COV; eauto.
+            { eapply tc_coherent_more; [| by apply COH'].
+              subst tc'. red. simpl. by rewrite COVEQ, ISSEQ. } 
+            specialize (SB_COV x). specialize_full SB_COV; [by vauto| ]. 
+            rewrite TC' in SB_COV. apply COVEQ in SB_COV.
+            destruct SB_COV; vauto. }
+          
+          econstructor; auto; simpl. 
+          { econstructor; eauto. }
+          { red. right. red. splits; simpl; auto.
+            apply issuable_next_w; auto.
+            { eapply tc_coherent_more; [| by apply COH'].
+              red. simpl. by rewrite COVEQ, ISSEQ. } 
+            split; auto. 
+            simpl. red. unfolder. splits; auto.
+            apply and_not_or. split; auto. intros ->. type_solver. }
+          red. left. red. splits.
+          3, 4: basic_solver. 
+          { simpl. apply and_not_or. split; auto. intros ->. type_solver. }
+          red. split.
+          { split; auto. }
+          repeat left. split; auto. basic_solver. }
+  Admitted. 
+             
 
   Lemma trav_step_closures_isim WF
         (tc tc': trav_config) 
@@ -228,15 +381,15 @@ Module SimTravClosure.
     assert (forall tc C1 I1 C2 I2
               (COV: covered tc ≡₁ C1 ∪₁ C2)
               (ISS: issued tc ≡₁ I1 ∪₁ I2),
-               tc = trav_conf_union (mkTC C1 I1) (mkTC C2 I2)) as TCU_HELPER.
-    { ins. unfold trav_conf_union. apply trav_config_eq_helper; simpl; auto. }
+               tc = (mkTC C1 I1) ⊔ (mkTC C2 I2)) as TCU_HELPER.
+    { ins. unfold trav_config_union. apply trav_config_eq_helper; simpl; auto. }
     red in TRAV_STEP. desc. red in TRAV_STEP. des.
     { pose proof (lab_rwf lab e) as LABe. des.
       { right. exists (tid e).
 
         (* destruct tc as [C I], tc' as [C' I']. simpl in *. *)
         remember (mkTC (eq e) ∅) as tc''. 
-        assert (tc' = trav_conf_union tc tc'') as TC'_UNION.
+        assert (tc' = tc ⊔ tc'') as TC'_UNION.
         { subst tc''. apply trav_config_eq_helper; simpl; auto.
           generalize ISSEQ. basic_solver. }
         rewrite TC'_UNION, stc_tcu_distribute.
@@ -253,22 +406,30 @@ Module SimTravClosure.
             2: { apply set_subset_empty_r. type_solver. }
             basic_solver. 
           }
-        }
+        }        
 
         rewrite TC''. rewrite !stc_alt. simpl.
         remember ({| covered := Cclos tc; issued := Iclos tc |}) as tcc.
+
+        destruct (classic (dom_rel rmw e)) as [RMWr | NRMWr].
+        2: { rewrite tcu_assoc. rewrite tcu_symm with (tc1 := tcc), <- tcu_assoc.
+             eapply isim_trav_step_mon_tcu. 
+
+
+        
         forward eapply eq_trans as TC''_UNION; [apply TC''| | ]. 
         { eapply TCU_HELPER; simpl; [reflexivity| ]. 
           symmetry. apply set_union_empty_l. }
-        rewrite <- TC'', TC''_UNION. 
+        rewrite <- TC'', TC''_UNION.
+
          
         
 
 
         rewrite !stc_alt.
         destruct tc as [C I], tc' as [C' I']. simpl in *.
-        (* unfold trav_conf_union, Iclos, Cclos. *)
-        unfold trav_conf_union. 
+        (* unfold trav_config_union, Iclos, Cclos. *)
+        unfold trav_config_union. 
         erewrite trav_config_eq_helper'. 
         2: { simpl. rewrite COVEQ, ISSEQ. reflexivity. }
         2: { simpl. rewrite ISSEQ, COVEQ. reflexivity. }
